Added DepositSpec and enforsed check for amount

verification/src/investments.dfy
@@ -9,7 +9,7 @@ module Investments {
     /**
       * Returns a new InvestmentAmount with the claimed field increased by the specified amount.
       *
-      * @param:: amountToAdd - a positive amount to add to the current claimed investment.
+      * @param: amountToAdd - a positive amount to add to the current claimed investment.
       *
       * @requires: amountToAdd > 0
       * @ensures: result.claimed == this.claimed + amountToAdd
@@ -20,6 +20,14 @@ module Investments {
       ensures result.claimed == this.claimed + amountToAdd
     {
       this.(claimed := this.claimed + amountToAdd)
+    }
+
+    function AddToAmountAndWeight(amount: nat, weight: nat): (result: InvestmentAmount)
+      requires amount > 0 && weight > 0
+      ensures result.amount == this.amount + amount
+      ensures result.weight == this.weight + weight
+    {
+      this.(amount := this.amount + amount, weight := this.weight + weight)
     }
   }
 }
