verification/src/deposit.dfy
@@ -1,0 +1,106 @@
+
+module Deposit {
+  import opened Prelude
+  import opened Config
+  import opened Investments
+  import opened Discounts
+
+  /**
+    * Calculates the assets based on the amount and price fraction.
+    *
+    * @param amount - base amount (nat)
+    * @param depositToken - price denominator (nat)
+    * @param saleToken - price numerator (nat)
+    * @returns assets (nat)
+    */
+  function CalculateAssets(amount: nat, depositToken: nat, saleToken: nat): nat
+    requires depositToken > 0 && saleToken > 0
+    // ensures CalculateAssets(amount, depositToken, saleToken) == (amount * saleToken) / depositToken
+  {
+    (amount * saleToken) / depositToken
+  }
+
+  /**
+    * Reverts the asset calculation to get the amount based on the price fraction.
+    *
+    * @param amount - base amount (nat)
+    * @param depositToken - price denominator (nat)
+    * @param saleToken - price numerator (nat)
+    * @returns reverted amount (nat)
+    */
+  function CalculateAssetsRevert(amount: nat, depositToken: nat, saleToken: nat): nat
+    requires depositToken > 0 && saleToken > 0
+    ensures CalculateAssetsRevert(amount, depositToken, saleToken) == (amount * depositToken) / saleToken
+  {
+    (amount * depositToken) / saleToken
+  }
+
+  ghost function DepositPriceDiscovery(
+    amount: nat,
+    weight: nat,
+    totalDeposited: nat,
+    totalSoldTokens: nat,
+    time: nat,
+    investment: InvestmentAmount
+  ): (InvestmentAmount, nat, nat)
+    requires amount > 0 && weight > 0
+    ensures DepositPriceDiscovery(amount, weight, totalDeposited, totalSoldTokens, time, investment) == (investment.AddToAmountAndWeight(amount, weight), totalDeposited + amount, totalSoldTokens + weight)
+  {
+    var newInvestment := investment.AddToAmountAndWeight(amount, weight);
+    var newTotalDeposited := totalDeposited + amount;
+    var newTotalSold := totalSoldTokens + weight;
+    (newInvestment, newTotalDeposited, newTotalSold)
+  }
+
+  /**
+    * Specification function for deposit logic.
+    *
+    * @param cfg - launchpad config
+    * @param amount - deposit amount
+    * @param totalDeposited - current total deposited
+    * @param totalSoldTokens - current total sold tokens
+    * @param time - current timestamp
+    * @param investment - current investment    
+    * @returns tuple: (newInv, newTotalDeposited, newTotalSoldTokens, refund)
+    */
+  ghost function DepositSpec(
+    cfg: Config,
+    amount: nat,
+    totalDeposited: nat,
+    totalSoldTokens: nat,
+    time: nat,
+    investment: InvestmentAmount
+  ): (InvestmentAmount, nat, nat, nat)
+    requires cfg.ValidConfig()
+    requires amount > 0
+    requires totalSoldTokens <= cfg.saleAmount
+    ensures cfg.mechanic.PriceDiscovery? ==> var (_, _, _, refund) := DepositSpec(cfg, amount, totalDeposited, totalSoldTokens, time, investment); refund == 0
+  {
+    var weight := cfg.CalculateWeightedAmountSpec(amount, time);
+    assert weight > 0;
+
+    if cfg.mechanic.FixedPrice? then
+      var assets := CalculateAssets(weight, cfg.mechanic.depositTokenAmount, cfg.mechanic.saleTokenAmount);
+      var newWeight := investment.weight + assets;
+      var newTotalSold := totalSoldTokens + assets;
+      if newTotalSold > cfg.saleAmount then
+        var assetsExcess := newTotalSold - cfg.saleAmount;
+        var remain := CalculateAssetsRevert(assetsExcess,cfg.mechanic.depositTokenAmount, cfg.mechanic.saleTokenAmount);
+        var refund := cfg.CalculateOriginalAmountSpec(remain, time);
+
+        assert assetsExcess <= assets;
+        assume {:axiom} refund <= amount;
+
+        var newInvestment := InvestmentAmount(investment.amount + amount - refund, investment.weight + assets - assetsExcess, investment.claimed);
+        var newTotalDeposited: nat := totalDeposited + amount - refund;
+        (newInvestment, newTotalDeposited, cfg.saleAmount, refund)
+      else
+        var newInvestment := InvestmentAmount(investment.amount + amount, investment.weight + assets, investment.claimed);
+        var newTotalDeposited := totalDeposited + amount;
+        (newInvestment, newTotalDeposited, newTotalSold, 0)
+    else
+      var (newInvestment, newTotalDeposited, newTotalSold) := DepositPriceDiscovery(amount, weight, totalDeposited, totalSoldTokens, time, investment);
+      (newInvestment, newTotalDeposited, newTotalSold, 0)
+  }
+}
+
