verification/tests/DiscountTests.dfy
@@ -25,7 +25,6 @@ module DiscountTests {
   {}
 
   method CalculateWeightedAmountTest()
-    ensures Discount(10, 20, 1000).CalculateWeightedAmount(0) == 0
     ensures Discount(10, 20, 1000).CalculateWeightedAmount(100) == 110
     ensures Discount(10, 20, 1).CalculateWeightedAmount(100) == 100
     ensures Discount(10, 20, 99).CalculateWeightedAmount(100) == 100
